Verify StandardLibrary, begin writing/updating unit tests

src/StandardLibrary/StandardLibrary.dfy
@@ -48,8 +48,8 @@ module {:extern "STL"} StandardLibrary {
   function method RequireEqual<T(==)>(expected: T, actual: T): (r: Result<()>) 
       ensures r.Success? ==> expected == actual
   {
-    // TODO: Use RequireWithMessage when it is possible to call ToString on an arbitrary type
-    Require(expected == actual)
+    // TODO: Report message similar to "Expected ___ but got ___"
+    RequireWithMessage(expected == actual, "Failed equality")
   }
   
   function method Require(b: bool): (r: Result<()>) 
@@ -79,64 +79,18 @@ module {:extern "STL"} StandardLibrary {
     decreases |s|
   {
     var i := Find(s, delim, 0);
-    if i.Some? then [s[..i.get]] + Split(s[i.get+1..], delim) else [s]
-  }
-
-  lemma WillSplitOnDelim<T>(s: seq<T>, delim: T, head: seq<T>)
-    requires head < s  // head is a prefix of s
-    requires delim !in head && s[|head|] == delim
-    ensures Split(s, delim) == [head] + Split(s[|head|+1..], delim)
-  {
-    calc {
-      Split(s, delim);
-    ==  // def. Split
-      var i := Find(s, delim, 0);
-      if i.Some? then [s[..i.get]] + Split(s[i.get+1..], delim) else [s];
-    ==  { FindLocatesElem(s, delim, 0, |head|); }
-      [s[..|head|]] + Split(s[|head|+1..], delim);
-    ==  { assert s[..|head|] == head; }
-      [head] + Split(s[|head|+1..], delim);
-    }
-  }
-
-  lemma WillNotSplitWithOutDelim<T>(s: seq<T>, delim: T)
-    requires delim !in s
-    ensures Split(s, delim) == [s]
-  {
-    calc {
-      Split(s, delim);
-    ==  // def. Split
-      var i := Find(s, delim, 0);
-      if i.Some? then [s[..i.get]] + Split(s[i.get+1..], delim) else [s];
-    ==  { FindLocatesElem(s, delim, 0, |s|); }
-      [s];
-    }
+    if i.Some? then [s[..i.get]] + Split(s[(i.get + 1)..], delim) else [s]
   }
 
   function method Find<T(==)>(s: seq<T>, c: T, i: nat): (index: Option<nat>)
     requires i <= |s|
-    ensures index.Some? ==> i <= index.get
-                         && index.get < |s| && s[index.get] == c
-                         && c !in s[i..index.get]
+    ensures index.Some? ==>  i <= index.get < |s| && s[index.get] == c && c !in s[i..index.get]
     ensures index.None? ==> c !in s[i..]
     decreases |s| - i
   {
     if i == |s| then None
     else if s[i] == c then Some(i)
     else Find(s, c, i + 1)
-  }
-
-  lemma FindLocatesElem<T>(s: seq<T>, c: T, start: nat, hereItIs: nat)
-    requires start <= hereItIs <= |s|
-    requires forall i :: start <= i < hereItIs ==> s[i] != c
-    requires hereItIs == |s| || s[hereItIs] == c
-    ensures Find(s, c, start) == if hereItIs == |s| then None else Some(hereItIs)
-    decreases hereItIs - start
-  {
-  }
-
-  predicate StringIs8Bit(s: string) {
-    forall i :: 0 <= i < |s| ==> s[i] < 256 as char
   }
 
   function Fill<T>(value: T, n: nat): seq<T>
@@ -154,221 +108,16 @@ module {:extern "STL"} StandardLibrary {
     a := new T[|s|](i requires 0 <= i < |s| => s[i]);
   }
 
-  method StringToByteArray(s: string) returns (a: array<uint8>)
-    ensures fresh(a) && a.Length <= 2 * |s|
-  {
-    // Assume all 8-bit characters for now
-    a := new uint8[|s|];
-    forall i | 0 <= i < |s| {
-      a[i] := (s[i] as int % 256) as uint8;
-    }
-  }
-
-  class mut<T> {
-    var x: T
-    constructor (y: T)
-      ensures x == y
-    {
-      x := y;
-    }
-    method put(y: T)
-      modifies this
-      ensures x == y
-    {
-      x := y;
-    }
-    function method get(): (y: T)
-      reads this
-      ensures y == x
-    {
-      x
-    }
-  }
-
-  predicate method uniq<T(==)>(s: seq<T>) {
-    if s == [] then true else if s[0] in s[1..] then false else uniq(s[1..])
-  }
-
-  lemma uniq_idxP<T>(s: seq<T>)
-    ensures uniq(s) <==> (forall i, j :: 0 <= i < j < |s| ==> s[i] != s[j])
-  {
-  }
-
-  // TODO
-  lemma {:axiom} uniq_multisetP<T>(s: seq<T>)
-    ensures uniq(s) <==> (forall x :: x in s ==> multiset(s)[x] == 1)
-
-  function method sum<T>(s: seq<T>, f: T -> int): int {
-    if s == [] then 0 else f(s[0]) + sum(s[1..], f)
-  }
-
-  lemma {:axiom} sum_perm<T>(s: seq <T>, s': seq<T>, f: T -> int)
-    requires multiset(s) == multiset(s')
-    ensures sum(s, f) == sum(s', f)
-
-
-  function count<T>(s: seq<T>, x: T): int {
-    if s == [] then 0 else (if s[0] == x then 1 else 0) + count(s[1..], x)
-  }
-
-  lemma count_ge0<T>(s: seq<T>, x: T)
-    ensures 0 <= count(s, x)
-  {
-    if s == [] {
-    } else {
-      assert count(s, x) == (if x == s[0] then 1 else 0) + count(s[1..], x);
-      count_ge0(s[1..], x);
-    }
-  }
-
-  lemma count_nil<T>(x: T)
-    ensures count([], x) == 0
-  { }
-
-  lemma in_count_gt0P<T>(s: seq<T>, x: T)
-    ensures (x in s) <==> (count(s, x) > 0)
-  {
-    if s != [] && s[0] == x {
-      count_ge0(s[1..], x);
-    }
-  }
-
-  lemma count_idx_gt0P<T>(s: seq<T>, i: int)
-    requires 0 <= i < |s|
-    ensures count(s, s[i]) > 0
-  {
-    assert s[i] in s;
-    in_count_gt0P(s, s[i]);
-  }
-
-  lemma count_eq0P<T>(s: seq<T>, x: T)
-    ensures (x !in s) <==> (count(s, x) == 0)
-  {
-    if s != [] && s[0] == x {
-      assert s[0] in s;
-      assert x in s;
-      count_ge0(s[1..], x);
-    }
-  }
-
-  lemma uniq_count_le1<T>(s: seq<T>, x: T)
-    requires uniq(s)
-    ensures count(s, x) <= 1
-  {
-    if s != [] && s[0] == x {
-      assert (s[0] !in s[1..]);
-      count_eq0P(s[1..], x);
-    }
-  }
-
-  lemma multiset_seq_count<T>(s: seq<T>, x: T)
-    ensures multiset(s)[x] == count(s, x)
-  {
-    if s == [] {
-    } else {
-      assert s == [s[0]] + s[1..];
-      assert multiset(s) == multiset{s[0]} + multiset(s[1..]);
-      assert multiset(s)[x] == multiset{s[0]}[x] + multiset(s[1..])[x];
-      multiset_seq_count(s[1..], x);
-    }
-  }
-
-  // TODO
-  lemma {:axiom} multiset_seq_eq1<T>(s: seq<T>)
-    requires forall i, j :: 0 <= i < j < |s| ==> s[i] != s[j]
-    ensures forall x :: x in multiset(s) ==> multiset(s)[x] == 1
-
-  // TODO
-  lemma {:axiom} multiset_of_seq_dup<T>(s: seq<T>, i: int, j: int)
-    requires 0 <= i < j < |s|
-    requires s[i] == s[j]
-    ensures multiset(s)[s[i]] > 1
-
-  lemma multiset_of_seq_gt0P<T>(s: seq<T>, x: T)
-    requires multiset(s)[x] > 0
-    ensures exists i :: 0 <= i < |s| && s[i] == x
-  { }
-
-  // TODO
-  lemma {:axiom} seq_dup_multset<T>(s: seq<T>, x: T)
-    requires multiset(s)[x] > 1
-    ensures exists i, j :: 0 <= i < j < |s| && s[i] == s[j]
-
-
-  lemma eq_multiset_seq_memP<T>(s: seq<T>, s': seq<T>, x: T)
-    requires multiset(s) == multiset(s')
-    ensures (x in s) == (x in s')
-  {
-    if x in s {
-      assert x in multiset(s);
-      assert x in multiset(s');
-      assert x in s';
-    }
-    else {
-      assert x !in multiset(s);
-      assert x !in multiset(s');
-      assert x !in s';
-    }
-  }
-
-  function method MapSeq<S, T>(s: seq<S>, f: S ~> T): seq<T>
-    requires forall i :: 0 <= i < |s| ==> f.requires(s[i])
-    reads set i,o | 0 <= i < |s| && o in f.reads(s[i]) :: o
-    decreases s
-  {
-    if s == [] then [] else [f(s[0])] + MapSeq(s[1..], f)
-  }
-
-  function method FlattenSeq<T>(s: seq<seq<T>>): seq<T> {
-    if s == [] then [] else s[0] + FlattenSeq(s[1..])
-  }
-
-  predicate method uniq_fst<S(==), T(==)>(s: seq<(S, T)>) {
-    uniq(MapSeq(s, (x: (S, T)) => x.0))
-  }
-
-
-  // TODO
-  lemma {:axiom} uniq_fst_uniq<S, T>(s: seq<(S,T)>)
-    requires uniq_fst(s)
-    ensures uniq(s)
-
-  // TODO
-  lemma {:axiom} uniq_fst_idxP<S, T>(s: seq<(S, T)>)
-    requires uniq_fst(s)
-    ensures forall i, j :: 0 <= i < j < |s| ==> s[i].0 != s[j].0
-
   function method min(a: int, b: int): int {
     if a < b then a else b
   }
-
-  method values<A,B>(m: map<A,B>) returns (vals: seq<B>) {
-    var keys := m.Keys;
-    vals := [];
-    while keys != {}
-      invariant |keys| + |vals| == |m.Keys|
-      decreases keys
-    {
-      var a :| a in keys;
-      keys := keys - {a};
-      vals := vals + [m[a]];
-    }
-  }
-
-  lemma {:axiom} eq_multiset_eq_len<T>(s: seq<T>, s': seq<T>)
-    requires multiset(s) == multiset(s')
-    ensures |s| == |s'|
-
-  predicate method UInt8Less(a: uint8, b: uint8) { a < b }
-  predicate method NatLess(a: nat, b: nat)  { a < b }
-  predicate method IntLess(a: int, b: int)  { a < b }
 
   /*
    * Lexicographic comparison of sequences.
    *
    * Given two sequences `a` and `b` and a strict (that is, irreflexive)
-   * ordering `less` on the elements of these sequences, `LexCmpSeqs(a, b, less)`
-   * says whether or not `a` is lexicographically "less than or equal to" `b`.
+   * ordering `less` on the elements of these sequences, determine whether or not
+   * `a` is lexicographically "less than or equal to" `b`.
    *
    * `a` is lexicographically "less than or equal to" `b` holds iff
    *   there exists a `k` such that
@@ -385,10 +134,8 @@ module {:extern "STL"} StandardLibrary {
   predicate method LexicographicLessOrEqualAux<T(==)>(a: seq<T>, b: seq<T>, less: (T, T) -> bool, lengthOfCommonPrefix: nat)
     requires 0 <= lengthOfCommonPrefix <= |a|
   {
-    lengthOfCommonPrefix <= |b| &&
-    (forall i :: 0 <= i < lengthOfCommonPrefix ==> a[i] == b[i]) &&
-    (lengthOfCommonPrefix == |a| ||
-     (lengthOfCommonPrefix < |b| && less(a[lengthOfCommonPrefix], b[lengthOfCommonPrefix])))
+    lengthOfCommonPrefix <= |b| && (forall i :: 0 <= i < lengthOfCommonPrefix ==> a[i] == b[i]) &&
+      (lengthOfCommonPrefix == |a| || (lengthOfCommonPrefix < |b| && less(a[lengthOfCommonPrefix], b[lengthOfCommonPrefix])))
   }
 
   /*
@@ -451,14 +198,14 @@ module {:extern "STL"} StandardLibrary {
   }
 
   lemma FilterIsDistributive<T>(s: seq<T>, s': seq<T>, f: T -> bool)
-    ensures Filter(s+s', f) == Filter(s,f) + Filter(s',f)
+    ensures Filter(s + s', f) == Filter(s, f) + Filter(s', f)
   {
     if s == [] {
       assert s + s' == s';
     } else {
       FilterIsDistributive<T>(s[1..], s', f);
       assert s + s' == [s[0]] + (s[1..] + s');
-      assert Filter(s+s', f) == Filter(s,f) + Filter(s',f);
+      assert Filter(s + s', f) == Filter(s, f) + Filter(s', f);
     }
   }
 }
